language/stackless-bytecode/tree_heap/output.bpl
@@ -4,7 +4,7 @@ type LocalName;
 type Address = int;
 type ByteArray;
 type String;
-
+type Location = int;
 type {:datatype} Edge;
 function {:constructor} Field(f: FieldName): Edge;
 function {:constructor} Index(i: int): Edge;
@@ -22,25 +22,29 @@ function {:constructor} Address(a: Address): Value;
 function {:constructor} ByteArray(b: ByteArray): Value;
 function {:constructor} Str(a: String): Value;
 function {:constructor} Map(m: [Edge]Value): Value;
+function {:constructor} Vector(v: [Edge]Value, l: int): Value;
 
 const DefaultMap: [Edge]Value;
 
 type {:datatype} Reference;
-function {:constructor} Reference(rt: RefType, p: Path): Reference;
+function {:constructor} Reference(rt: RefType, p: Path, l: Location): Reference;
 
 type {:datatype} RefType;
 function {:constructor} Global(a: Address, t: TypeName): RefType;
-function {:constructor} Local(l: int): RefType;
+function {:constructor} Local(): RefType;
 
 type {:datatype} TypeStore;
-function {:constructor} TypeStore(domain: [TypeName]bool, contents: [TypeName]Value): TypeStore;
+function {:constructor} TypeStore(domain: [TypeName]bool, contents: [TypeName]Location): TypeStore;
 
 type {:datatype} GlobalStore;
 function {:constructor} GlobalStore(domain: [Address]bool, contents: [Address]TypeStore): GlobalStore;
 
+type {:datatype} Memory;
+function {:constructor} Memory(domain: [Location]bool, contents: [Location]Value): Memory;
+
 var gs : GlobalStore;
-var ls : [int]Value;
-var ls_size : int;
+var m : Memory;
+var m_size : int;
 
 procedure {:inline 1} Exists(address: Value, t: TypeName) returns (dst: Value)
 requires is#Address(address);
@@ -56,8 +60,10 @@ procedure {:inline 1} MoveToSender(t: TypeName, v: Value)
     assert domain#GlobalStore(gs)[a];
     ts := contents#GlobalStore(gs)[a];
     assert !domain#TypeStore(ts)[t];
-    ts := TypeStore(domain#TypeStore(ts)[t := true], contents#TypeStore(ts)[t := v]);
+    ts := TypeStore(domain#TypeStore(ts)[t := true], contents#TypeStore(ts)[t := m_size]);
     gs := GlobalStore(domain#GlobalStore(gs), contents#GlobalStore(gs)[a := ts]);
+    m := Memory(domain#Memory(m)[m_size := true], contents#Memory(m)[m_size := v]);
+    m_size := m_size + 1;
 }
 
 procedure {:inline 1} MoveFrom(address: Value, t: TypeName) returns (dst: Value)
@@ -65,11 +71,15 @@ requires is#Address(address);
 {
     var a: Address;
     var ts: TypeStore;
+    var l: Location;
     a := a#Address(address);
     assert domain#GlobalStore(gs)[a];
     ts := contents#GlobalStore(gs)[a];
     assert domain#TypeStore(ts)[t];
-    dst := contents#TypeStore(ts)[t];
+    l := contents#TypeStore(ts)[t];
+    assert domain#Memory(m)[l];
+    dst := contents#Memory(m)[l];
+    m := Memory(domain#Memory(m)[l := false], contents#Memory(m));
     ts := TypeStore(domain#TypeStore(ts)[t := false], contents#TypeStore(ts));
     gs := GlobalStore(domain#GlobalStore(gs), contents#GlobalStore(gs)[a := ts]);
 }
@@ -80,16 +90,19 @@ requires is#Address(address);
     var a: Address;
     var v: Value;
     var ts: TypeStore;
+    var l: Location;
     a := a#Address(address);
     assert domain#GlobalStore(gs)[a];
     ts := contents#GlobalStore(gs)[a];
     assert domain#TypeStore(ts)[t];
-    dst := Reference(Global(a, t), Path(DefaultPath, 0));
+    l := contents#TypeStore(ts)[t];
+    assert domain#Memory(m)[l];
+    dst := Reference(Global(a, t), Path(DefaultPath, 0), l);
 }
 
 procedure {:inline 1} BorrowLoc(l: int) returns (dst: Reference)
 {
-    dst := Reference(Local(l), Path(DefaultPath, 0));
+    dst := Reference(Local(), Path(DefaultPath, 0), l);
 }
 
 procedure {:inline 1} BorrowField(src: Reference, f: FieldName) returns (dst: Reference)
@@ -98,9 +111,8 @@ procedure {:inline 1} BorrowField(src: Reference, f: FieldName) returns (dst: Re
     var size: int;
     p := p#Reference(src);
     size := size#Path(p);
-	p := Path(p#Path(p)[size := Field(f)], size+1);
-    dst := Reference(rt#Reference(src), p);
-
+	  p := Path(p#Path(p)[size := Field(f)], size+1);
+    dst := Reference(rt#Reference(src), p, l#Reference(src));
 }
 
 procedure {:inline 1} WriteRef(to: Reference, new_v: Value)
@@ -109,20 +121,21 @@ procedure {:inline 1} WriteRef(to: Reference, new_v: Value)
     var ts: TypeStore;
     var t: TypeName;
     var v: Value;
+    var l: Location;
     if (is#Global(rt#Reference(to))) {
         a := a#Global(rt#Reference(to));
         assert domain#GlobalStore(gs)[a];
         ts := contents#GlobalStore(gs)[a];
         t := t#Global(rt#Reference(to));
         assert domain#TypeStore(ts)[t];
-        v := contents#TypeStore(ts)[t];
+        l := l#Reference(to);
+        v := contents#Memory(m)[l];
         call v := UpdateValueMax(p#Reference(to), 0, v, new_v);
-        ts := TypeStore(domain#TypeStore(ts), contents#TypeStore(ts)[t := v]);
-        gs := GlobalStore(domain#GlobalStore(gs), contents#GlobalStore(gs)[a := ts]);
+        m := Memory(domain#Memory(m), contents#Memory(m)[l := v]);
     } else {
-        v := ls[l#Local(rt#Reference(to))];
+        v := contents#Memory(m)[l#Reference(to)];
         call v := UpdateValueMax(p#Reference(to), 0, v, new_v);
-        ls := ls[l#Local(rt#Reference(to)) := v];
+        m := Memory(domain#Memory(m), contents#Memory(m)[l#Reference(to) := v]);
     }
 }
 
@@ -137,9 +150,9 @@ procedure {:inline 1} ReadRef(from: Reference) returns (v: Value)
         ts := contents#GlobalStore(gs)[a];
         t := t#Global(rt#Reference(from));
         assert domain#TypeStore(ts)[t];
-        call v := ReadValueMax(p#Reference(from), 0, contents#TypeStore(ts)[t]);
+        call v := ReadValueMax(p#Reference(from), 0, contents#Memory(m)[contents#TypeStore(ts)[t]]);
     } else {
-        call v := ReadValueMax(p#Reference(from), 0, ls[l#Local(rt#Reference(from))]);
+        call v := ReadValueMax(p#Reference(from), 0, contents#Memory(m)[l#Reference(from)]);
     }
 }
 
@@ -249,6 +262,26 @@ procedure {:inline 1} Not(src: Value) returns (dst: Value)
 {
     assert is#Boolean(src);
     dst := Boolean(!b#Boolean(src));
+}
+
+procedure {:inline 1} Eq(src1: Value, src2: Value) returns (dst: Value)
+{
+    dst := Boolean(src1 == src2);
+}
+
+procedure {:inline 1} Neq(src1: Value, src2: Value) returns (dst: Value)
+{
+    dst := Boolean(src1 != src2);
+}
+
+procedure {:inline 1} Eq_Vector_T(src1: Value, src2: Value) returns (dst: Value)
+{
+    dst := Boolean(src1 == src2);
+}
+
+procedure {:inline 1} Neq_Vector_T(src1: Value, src2: Value) returns (dst: Value)
+{
+    dst := Boolean(src1 != src2);
 }
 
 procedure {:inline 1} Eq_int(src1: Value, src2: Value) returns (dst: Value)
@@ -366,43 +399,163 @@ procedure {:inline 1} GetTxnGasUnitPrice() returns (ret_gas_unit_price: Value)
   ret_gas_unit_price := Integer(gas_unit_price#Transaction_cons(txn));
 }
 
+procedure {:inline 1} Vector_empty() returns (v: Value) {
+    v := Vector(DefaultMap, 0);
+}
+
+procedure {:inline 1} Vector_is_empty(r: Reference) returns (b: Value) {
+    var v: Value;
+    call v := ReadRef(r);
+    b := Boolean(l#Vector(v) == 0);
+}
+
+procedure {:inline 1} Vector_push_back(r: Reference, val: Value) {
+    var old_v: Value;
+    var old_len: int;
+    call old_v := ReadRef(r);
+    old_len := l#Vector(old_v);
+    call WriteRef(r, Vector(v#Vector(old_v)[Index(old_len) := val], old_len+1));
+}
+
+procedure {:inline 1} Vector_pop_back(r: Reference) returns (e: Value){
+    var v: Value;
+    var old_len: int;
+    call v := ReadRef(r);
+    old_len := l#Vector(v);
+    e := v#Vector(v)[Index(old_len-1)];
+    call WriteRef(r, Vector(v#Vector(v), old_len-1));
+}
+
+procedure {:inline 1} Vector_append(r: Reference, other_v: Value) {
+    var v: Value;
+    var old_len: int;
+    var other_len: int;
+    var result: Value;
+    call v := ReadRef(r);
+    old_len := l#Vector(v);
+    other_len := l#Vector(other_v);
+    result := Vector(
+        (lambda e:Edge ::
+            if i#Index(e) < old_len then
+		        v#Vector(v)[e]
+		    else
+		        v#Vector(other_v)[Index(i#Index(e) - old_len)]
+        ),
+	    old_len + other_len);
+    call WriteRef(r, result);
+}
+
+procedure {:inline 1} Vector_reverse(r: Reference) {
+    var v: Value;
+    var result: Value;
+    var len: int;
+
+    call v := ReadRef(r);
+    len := l#Vector(v);
+    result := Vector(
+        (lambda e:Edge ::
+            v#Vector(v)[Index(len-i#Index(e)-1)]
+        ),
+	    len);
+    call WriteRef(r, result);
+}
+
+procedure {:inline 1} Vector_length(r: Reference) returns (l: Value) {
+    var v: Value;
+    call v := ReadRef(r);
+    l := Integer(l#Vector(v));
+}
+
+procedure {:inline 1} Vector_borrow(src: Reference, index: Value) returns (dst: Reference) {
+    var p: Path;
+    var size: int;
+    p := p#Reference(src);
+    size := size#Path(p);
+	  p := Path(p#Path(p)[size := Index(i#Integer(index))], size+1);
+    dst := Reference(rt#Reference(src), p, l#Reference(src));
+}
+
+procedure {:inline 1} Vector_borrow_mut(src: Reference, index: Value) returns (dst: Reference) {
+    var p: Path;
+    var size: int;
+    p := p#Reference(src);
+    size := size#Path(p);
+	  p := Path(p#Path(p)[size := Index(i#Integer(index))], size+1);
+    dst := Reference(rt#Reference(src), p, l#Reference(src));
+}
+
+procedure {:inline 1} Vector_destroy_empty(v: Value) {
+    assert (l#Vector(v) == 0);
+}
+
+procedure {:inline 1} Vector_swap(src: Reference, i: Value, j: Value) {
+    var i_val: Value;
+    var j_val: Value;
+    var i_ind: int;
+    var j_ind: int;
+    var v: Value;
+    i_ind := i#Integer(i);
+    j_ind := i#Integer(j);
+    call v := ReadRef(src);
+    assert (l#Vector(v) > i_ind && l#Vector(v) > j_ind);
+    i_val := v#Vector(v)[Index(i_ind)];
+    j_val := v#Vector(v)[Index(j_ind)];
+    v := Vector(v#Vector(v)[Index(i_ind) := j_val][Index(j_ind) := i_val], l#Vector(v));
+    call WriteRef(src, v);
+}
+
+procedure {:inline 1} Vector_get(src: Reference, i: Value) returns (e: Value) {
+    var i_ind: int;
+    var v: Value;
+    call v := ReadRef(src);
+    i_ind := i#Integer(i);
+    assert (i_ind < l#Vector(v));
+    e := v#Vector(v)[Index(i_ind)];
+}
+
+procedure {:inline 1} Vector_set(src: Reference, i: Value, e: Value) {
+    var i_ind: int;
+    var v: Value;
+    i_ind := i#Integer(i);
+    call v := ReadRef(src);
+    assert (l#Vector(v) > i_ind);
+    v := Vector(v#Vector(v)[Index(i_ind) := e], l#Vector(v));
+    call WriteRef(src, v);
+}
+
 
 // everything below is auto generated
 
-const unique Test3_T: TypeName;
-const unique Test3_T_f: FieldName;
-const unique Test3_T_g: FieldName;
+const unique Vector_T: TypeName;
+const unique Option_T: TypeName;
+const unique Option_T_v: FieldName;
 
-procedure {:inline 1} Pack_Test3_T(v0: Value, v1: Value) returns (v: Value)
+procedure {:inline 1} Pack_Option_T(v0: Value) returns (v: Value)
 {
-    assert is#Integer(v0);
-    assert is#Integer(v1);
-    v := Map(DefaultMap[Field(Test3_T_f) := v0][Field(Test3_T_g) := v1]);
+    assert is#Vector(v0);
+    v := Map(DefaultMap[Field(Option_T_v) := v0]);
 }
 
-procedure {:inline 1} Unpack_Test3_T(v: Value) returns (v0: Value, v1: Value)
+procedure {:inline 1} Unpack_Option_T(v: Value) returns (v0: Value)
 {
     assert is#Map(v);
-    v0 := m#Map(v)[Field(Test3_T_f)];
-    v1 := m#Map(v)[Field(Test3_T_g)];
+    v0 := m#Map(v)[Field(Option_T_v)];
 }
 
-procedure {:inline 1} Eq_Test3_T(v1: Value, v2: Value) returns (res: Value)
+procedure {:inline 1} Eq_Option_T(v1: Value, v2: Value) returns (res: Value)
 {
     var b0: Value;
-    var b1: Value;
     assert is#Map(v1) && is#Map(v2);
-    call b0 := Eq_int(m#Map(v1)[Field(Test3_T_f)], m#Map(v2)[Field(Test3_T_f)]);
-    call b1 := Eq_int(m#Map(v1)[Field(Test3_T_g)], m#Map(v2)[Field(Test3_T_g)]);
-    res := Boolean(true && b#Boolean(b0) && b#Boolean(b1));
+    call b0 := Eq_Vector_T(m#Map(v1)[Field(Option_T_v)], m#Map(v2)[Field(Option_T_v)]);
+    res := Boolean(true && b#Boolean(b0));
 }
 
-procedure {:inline 1} Neq_Test3_T(v1: Value, v2: Value) returns (res: Value)
+procedure {:inline 1} Neq_Option_T(v1: Value, v2: Value) returns (res: Value)
 {
     var res_val: Value;
     var res_bool: bool;
     assert is#Map(v1) && is#Map(v2);
-    call res_val := Eq_Test3_T(v1, v2);
+    call res_val := Eq_Option_T(v1, v2);
     res := Boolean(!b#Boolean(res_val));
 }
 
@@ -416,6 +569,19 @@ procedure {:inline 1} ReadValue0(p: Path, i: int, v: Value) returns (v': Value)
     }
 }
 
+procedure {:inline 1} ReadValue1(p: Path, i: int, v: Value) returns (v': Value)
+{
+    var e: Edge;
+    if (i == size#Path(p)) {
+        v' := v;
+    } else {
+        e := p#Path(p)[i];
+        v' := m#Map(v)[e];
+        if (is#Vector(v)) { v' := v#Vector(v)[e]; }
+        call v' := ReadValue0(p, i+1, v');
+    }
+}
+
 procedure {:inline 1} ReadValueMax(p: Path, i: int, v: Value) returns (v': Value)
 {
     var e: Edge;
@@ -424,7 +590,8 @@ procedure {:inline 1} ReadValueMax(p: Path, i: int, v: Value) returns (v': Value
     } else {
         e := p#Path(p)[i];
         v' := m#Map(v)[e];
-        call v' := ReadValue0(p, i+1, v');
+        if (is#Vector(v)) { v' := v#Vector(v)[e]; }
+        call v' := ReadValue1(p, i+1, v');
     }
 }
 
@@ -438,6 +605,21 @@ procedure {:inline 1} UpdateValue0(p: Path, i: int, v: Value, new_v: Value) retu
     }
 }
 
+procedure {:inline 1} UpdateValue1(p: Path, i: int, v: Value, new_v: Value) returns (v': Value)
+{
+    var e: Edge;
+    if (i == size#Path(p)) {
+        v' := new_v;
+    } else {
+        e := p#Path(p)[i];
+        v' := m#Map(v)[e];
+        if (is#Vector(v)) { v' := v#Vector(v)[e]; }
+        call v' := UpdateValue0(p, i+1, v', new_v);
+        if (is#Map(v)) { v' := Map(m#Map(v)[e := v']);}
+        if (is#Vector(v)) { v' := Vector(v#Vector(v)[e := v'], l#Vector(v));}
+    }
+}
+
 procedure {:inline 1} UpdateValueMax(p: Path, i: int, v: Value, new_v: Value) returns (v': Value)
 {
     var e: Edge;
@@ -446,290 +628,1046 @@ procedure {:inline 1} UpdateValueMax(p: Path, i: int, v: Value, new_v: Value) re
     } else {
         e := p#Path(p)[i];
         v' := m#Map(v)[e];
-        call v' := UpdateValue0(p, i+1, v', new_v);
-        v' := Map(m#Map(v)[e := v']);
+        if (is#Vector(v)) { v' := v#Vector(v)[e]; }
+        call v' := UpdateValue1(p, i+1, v', new_v);
+        if (is#Map(v)) { v' := Map(m#Map(v)[e := v']);}
+        if (is#Vector(v)) { v' := Vector(v#Vector(v)[e := v'], l#Vector(v));}
     }
 }
 
-procedure Test3_test3 (arg0: Value) returns ()
+procedure {:inline 1} Option_none () returns (ret0: Value)
 {
     // declare local variables
-    var t0: Value; // bool
-    var t1: Value; // Test3_T
-    var t2: Reference; // Test3_T_ref
-    var t3: Reference; // int_ref
-    var t4: Reference; // int_ref
-    var t5: Reference; // int_ref
-    var t6: Reference; // int_ref
-    var t7: Value; // int
-    var t8: Value; // int
-    var t9: Value; // int
-    var t10: Value; // int
-    var t11: Value; // Test3_T
-    var t12: Reference; // Test3_T_ref
-    var t13: Value; // bool
-    var t14: Reference; // Test3_T_ref
-    var t15: Reference; // int_ref
-    var t16: Reference; // Test3_T_ref
-    var t17: Reference; // int_ref
-    var t18: Value; // int
-    var t19: Reference; // int_ref
-    var t20: Value; // bool
-    var t21: Value; // bool
-    var t22: Reference; // Test3_T_ref
-    var t23: Reference; // int_ref
-    var t24: Reference; // Test3_T_ref
-    var t25: Reference; // int_ref
-    var t26: Value; // int
-    var t27: Reference; // int_ref
-    var t28: Reference; // Test3_T_ref
-    var t29: Reference; // int_ref
-    var t30: Reference; // Test3_T_ref
-    var t31: Reference; // int_ref
-    var t32: Reference; // int_ref
-    var t33: Value; // int
-    var t34: Reference; // int_ref
-    var t35: Value; // int
-    var t36: Value; // bool
-    var t37: Value; // int
-    var t38: Value; // int
-    var t39: Value; // bool
-    var t40: Value; // bool
-    var t41: Value; // int
-    var t42: Value; // int
-    var t43: Value; // int
-    var t44: Value; // bool
-    var t45: Value; // bool
-    var t46: Value; // int
-    var t47: Value; // int
-    var t48: Value; // int
-    var t49: Value; // bool
-    var t50: Value; // bool
-    var t51: Value; // int
-    var t52: Value; // int
-    var t53: Value; // int
-    var t54: Value; // bool
-    var t55: Value; // bool
-    var t56: Value; // int
+    var t0: Value; // Vector_T
+    var t1: Value; // Option_T
 
     var tmp: Value;
     var old_size: int;
     assume !abort_flag;
 
     // assume arguments are of correct types
-    assume is#Boolean(arg0);
 
-    old_size := ls_size;
-    ls_size := ls_size + 57;
-    ls[old_size+0] := arg0;
+    old_size := m_size;
+    m_size := m_size + 2;
 
     // bytecode translation starts here
-    call tmp := LdConst(0);
-    ls[old_size+9] := tmp;
+    call t0 := Vector_empty();
+    assume is#Vector(t0);
 
-    call tmp := LdConst(0);
-    ls[old_size+10] := tmp;
+    m := Memory(domain#Memory(m)[old_size+0 := true], contents#Memory(m)[old_size+0 := t0]);
 
-    assume is#Integer(ls[old_size+9]);
+    assume is#Vector(contents#Memory(m)[old_size+0]);
 
-    assume is#Integer(ls[old_size+10]);
+    call tmp := Pack_Option_T(contents#Memory(m)[old_size+0]);
+    m := Memory(domain#Memory(m)[1+old_size := true], contents#Memory(m)[1+old_size := tmp]);
 
-    call tmp := Pack_Test3_T(ls[old_size+9], ls[old_size+10]);
-    ls[old_size+11] := tmp;
+    ret0 := contents#Memory(m)[old_size+1];
+    return;
 
-    call tmp := CopyOrMoveValue(ls[old_size+11]);
-    ls[old_size+1] := tmp;
+}
 
-    call t12 := BorrowLoc(old_size+1);
+procedure Option_none_verify () returns (ret0: Value)
+{
+    call ret0 := Option_none();
+}
 
-    call t2 := CopyOrMoveRef(t12);
+procedure {:inline 1} Option_some (arg0: Value) returns (ret0: Value)
+{
+    // declare local variables
+    var t0: Value; // typeparam
+    var t1: Value; // Vector_T
+    var t2: Value; // Vector_T
+    var t3: Reference; // Vector_T_ref
+    var t4: Value; // typeparam
+    var t5: Value; // Vector_T
+    var t6: Value; // Option_T
 
-    call tmp := CopyOrMoveValue(ls[old_size+0]);
-    ls[old_size+13] := tmp;
+    var tmp: Value;
+    var old_size: int;
+    assume !abort_flag;
 
-    tmp := ls[old_size + 13];
-    if (!b#Boolean(tmp)) { goto Label_12; }
+    // assume arguments are of correct types
 
-    call t14 := CopyOrMoveRef(t2);
+    old_size := m_size;
+    m_size := m_size + 7;
+    m := Memory(domain#Memory(m)[0+old_size := true], contents#Memory(m)[0+old_size :=  arg0]);
 
-    call t15 := BorrowField(t14, Test3_T_f);
+    // bytecode translation starts here
+    call t2 := Vector_empty();
+    assume is#Vector(t2);
 
-    call t3 := CopyOrMoveRef(t15);
+    m := Memory(domain#Memory(m)[old_size+2 := true], contents#Memory(m)[old_size+2 := t2]);
 
-    goto Label_15;
+    call tmp := CopyOrMoveValue(contents#Memory(m)[old_size+2]);
+    m := Memory(domain#Memory(m)[1+old_size := true], contents#Memory(m)[1+old_size := tmp]);
 
-Label_12:
-    call t16 := CopyOrMoveRef(t2);
+    call t3 := BorrowLoc(old_size+1);
 
-    call t17 := BorrowField(t16, Test3_T_g);
+    call tmp := CopyOrMoveValue(contents#Memory(m)[old_size+0]);
+    m := Memory(domain#Memory(m)[4+old_size := true], contents#Memory(m)[4+old_size := tmp]);
 
-    call t3 := CopyOrMoveRef(t17);
+    call Vector_push_back(t3, contents#Memory(m)[old_size+4]);
 
-Label_15:
-    call tmp := LdConst(10);
-    ls[old_size+18] := tmp;
+    call tmp := CopyOrMoveValue(contents#Memory(m)[old_size+1]);
+    m := Memory(domain#Memory(m)[5+old_size := true], contents#Memory(m)[5+old_size := tmp]);
 
-    call t19 := CopyOrMoveRef(t3);
+    assume is#Vector(contents#Memory(m)[old_size+5]);
 
-    call WriteRef(t19, ls[old_size+18]);
+    call tmp := Pack_Option_T(contents#Memory(m)[old_size+5]);
+    m := Memory(domain#Memory(m)[6+old_size := true], contents#Memory(m)[6+old_size := tmp]);
 
-    call tmp := CopyOrMoveValue(ls[old_size+0]);
-    ls[old_size+20] := tmp;
+    ret0 := contents#Memory(m)[old_size+6];
+    return;
 
-    call tmp := Not(ls[old_size+20]);
-    ls[old_size+21] := tmp;
+}
 
-    tmp := ls[old_size + 21];
-    if (!b#Boolean(tmp)) { goto Label_25; }
+procedure Option_some_verify (arg0: Value) returns (ret0: Value)
+{
+    call ret0 := Option_some(arg0);
+}
 
-    call t22 := CopyOrMoveRef(t2);
+procedure {:inline 1} Option_unwrap_or (arg0: Value, arg1: Value) returns (ret0: Value)
+{
+    // declare local variables
+    var t0: Value; // Option_T
+    var t1: Value; // typeparam
+    var t2: Value; // Vector_T
+    var t3: Value; // Option_T
+    var t4: Value; // Vector_T
+    var t5: Reference; // Vector_T_ref
+    var t6: Value; // bool
+    var t7: Value; // typeparam
+    var t8: Reference; // Vector_T_ref
+    var t9: Value; // typeparam
 
-    call t23 := BorrowField(t22, Test3_T_f);
+    var tmp: Value;
+    var old_size: int;
+    assume !abort_flag;
 
-    call t4 := CopyOrMoveRef(t23);
+    // assume arguments are of correct types
+    assume is#Map(arg0);
 
-    goto Label_28;
+    old_size := m_size;
+    m_size := m_size + 10;
+    m := Memory(domain#Memory(m)[0+old_size := true], contents#Memory(m)[0+old_size :=  arg0]);
+    m := Memory(domain#Memory(m)[1+old_size := true], contents#Memory(m)[1+old_size :=  arg1]);
 
-Label_25:
-    call t24 := CopyOrMoveRef(t2);
+    // bytecode translation starts here
+    call tmp := CopyOrMoveValue(contents#Memory(m)[old_size+0]);
+    m := Memory(domain#Memory(m)[3+old_size := true], contents#Memory(m)[3+old_size := tmp]);
 
-    call t25 := BorrowField(t24, Test3_T_g);
+    call t4 := Unpack_Option_T(contents#Memory(m)[old_size+3]);
+    assume is#Vector(t4);
 
-    call t4 := CopyOrMoveRef(t25);
+    m := Memory(domain#Memory(m)[old_size+4 := true], contents#Memory(m)[old_size+4 := t4]);
 
-Label_28:
-    call tmp := LdConst(20);
-    ls[old_size+26] := tmp;
+    call tmp := CopyOrMoveValue(contents#Memory(m)[old_size+4]);
+    m := Memory(domain#Memory(m)[2+old_size := true], contents#Memory(m)[2+old_size := tmp]);
 
-    call t27 := CopyOrMoveRef(t4);
+    call t5 := BorrowLoc(old_size+2);
 
-    call WriteRef(t27, ls[old_size+26]);
+    call t6 := Vector_is_empty(t5);
+    assume is#Boolean(t6);
 
-    call t28 := CopyOrMoveRef(t2);
+    m := Memory(domain#Memory(m)[old_size+6 := true], contents#Memory(m)[old_size+6 := t6]);
 
-    call t29 := BorrowField(t28, Test3_T_f);
+    tmp := contents#Memory(m)[old_size + 6];
+if (!b#Boolean(tmp)) { goto Label_8; }
 
-    call t5 := CopyOrMoveRef(t29);
+    call tmp := CopyOrMoveValue(contents#Memory(m)[old_size+1]);
+    m := Memory(domain#Memory(m)[7+old_size := true], contents#Memory(m)[7+old_size := tmp]);
 
-    call t30 := CopyOrMoveRef(t2);
+    ret0 := contents#Memory(m)[old_size+7];
+    return;
 
-    call t31 := BorrowField(t30, Test3_T_g);
+Label_8:
+    call t8 := BorrowLoc(old_size+2);
 
-    call t6 := CopyOrMoveRef(t31);
+    call t9 := Vector_pop_back(t8);
 
-    call t32 := CopyOrMoveRef(t5);
+    m := Memory(domain#Memory(m)[old_size+9 := true], contents#Memory(m)[old_size+9 := t9]);
 
-    call tmp := ReadRef(t32);
-    assume is#Integer(tmp);
+    ret0 := contents#Memory(m)[old_size+9];
+    return;
 
-    ls[old_size+33] := tmp;
+}
 
-    call tmp := CopyOrMoveValue(ls[old_size+33]);
-    ls[old_size+7] := tmp;
+procedure Option_unwrap_or_verify (arg0: Value, arg1: Value) returns (ret0: Value)
+{
+    call ret0 := Option_unwrap_or(arg0, arg1);
+}
 
-    call t34 := CopyOrMoveRef(t6);
+procedure {:inline 1} Option_test_u64 () returns ()
+{
+    // declare local variables
+    var t0: Value; // Option_T
+    var t1: Value; // Option_T
+    var t2: Value; // Option_T
+    var t3: Value; // int
+    var t4: Value; // Option_T
+    var t5: Value; // Option_T
+    var t6: Value; // int
+    var t7: Value; // int
+    var t8: Value; // int
+    var t9: Value; // bool
+    var t10: Value; // bool
+    var t11: Value; // int
+    var t12: Value; // Option_T
+    var t13: Value; // int
+    var t14: Value; // int
+    var t15: Value; // int
+    var t16: Value; // bool
+    var t17: Value; // bool
+    var t18: Value; // int
 
-    call tmp := ReadRef(t34);
-    assume is#Integer(tmp);
+    var tmp: Value;
+    var old_size: int;
+    assume !abort_flag;
 
-    ls[old_size+35] := tmp;
+    // assume arguments are of correct types
 
-    call tmp := CopyOrMoveValue(ls[old_size+35]);
-    ls[old_size+8] := tmp;
+    old_size := m_size;
+    m_size := m_size + 19;
 
-    call tmp := CopyOrMoveValue(ls[old_size+0]);
-    ls[old_size+36] := tmp;
+    // bytecode translation starts here
+    call t2 := Option_none();
+    assume is#Map(t2);
 
-    tmp := ls[old_size + 36];
-    if (!b#Boolean(tmp)) { goto Label_60; }
+    m := Memory(domain#Memory(m)[old_size+2 := true], contents#Memory(m)[old_size+2 := t2]);
 
-    call tmp := CopyOrMoveValue(ls[old_size+7]);
-    ls[old_size+37] := tmp;
-
-    call tmp := LdConst(10);
-    ls[old_size+38] := tmp;
-
-    call tmp := Eq_int(ls[old_size+37], ls[old_size+38]);
-    ls[old_size+39] := tmp;
-
-    call tmp := Not(ls[old_size+39]);
-    ls[old_size+40] := tmp;
-
-    tmp := ls[old_size + 40];
-    if (!b#Boolean(tmp)) { goto Label_52; }
+    call tmp := CopyOrMoveValue(contents#Memory(m)[old_size+2]);
+    m := Memory(domain#Memory(m)[0+old_size := true], contents#Memory(m)[0+old_size := tmp]);
 
     call tmp := LdConst(42);
-    ls[old_size+41] := tmp;
+    m := Memory(domain#Memory(m)[3+old_size := true], contents#Memory(m)[3+old_size := tmp]);
+
+    call t4 := Option_some(contents#Memory(m)[old_size+3]);
+    assume is#Map(t4);
+
+    m := Memory(domain#Memory(m)[old_size+4 := true], contents#Memory(m)[old_size+4 := t4]);
+
+    call tmp := CopyOrMoveValue(contents#Memory(m)[old_size+4]);
+    m := Memory(domain#Memory(m)[1+old_size := true], contents#Memory(m)[1+old_size := tmp]);
+
+    call tmp := CopyOrMoveValue(contents#Memory(m)[old_size+0]);
+    m := Memory(domain#Memory(m)[5+old_size := true], contents#Memory(m)[5+old_size := tmp]);
+
+    call tmp := LdConst(0);
+    m := Memory(domain#Memory(m)[6+old_size := true], contents#Memory(m)[6+old_size := tmp]);
+
+    call t7 := Option_unwrap_or(contents#Memory(m)[old_size+5], contents#Memory(m)[old_size+6]);
+    assume is#Integer(t7);
+
+    m := Memory(domain#Memory(m)[old_size+7 := true], contents#Memory(m)[old_size+7 := t7]);
+
+    call tmp := LdConst(0);
+    m := Memory(domain#Memory(m)[8+old_size := true], contents#Memory(m)[8+old_size := tmp]);
+
+    call tmp := Eq(contents#Memory(m)[old_size+7], contents#Memory(m)[old_size+8]);
+    m := Memory(domain#Memory(m)[9+old_size := true], contents#Memory(m)[9+old_size := tmp]);
+
+    call tmp := Not(contents#Memory(m)[old_size+9]);
+    m := Memory(domain#Memory(m)[10+old_size := true], contents#Memory(m)[10+old_size := tmp]);
+
+    tmp := contents#Memory(m)[old_size + 10];
+if (!b#Boolean(tmp)) { goto Label_14; }
+
+    call tmp := LdConst(10);
+    m := Memory(domain#Memory(m)[11+old_size := true], contents#Memory(m)[11+old_size := tmp]);
 
     assert false;
 
-Label_52:
-    call tmp := CopyOrMoveValue(ls[old_size+8]);
-    ls[old_size+42] := tmp;
+Label_14:
+    call tmp := CopyOrMoveValue(contents#Memory(m)[old_size+1]);
+    m := Memory(domain#Memory(m)[12+old_size := true], contents#Memory(m)[12+old_size := tmp]);
 
-    call tmp := LdConst(20);
-    ls[old_size+43] := tmp;
+    call tmp := LdConst(0);
+    m := Memory(domain#Memory(m)[13+old_size := true], contents#Memory(m)[13+old_size := tmp]);
 
-    call tmp := Eq_int(ls[old_size+42], ls[old_size+43]);
-    ls[old_size+44] := tmp;
+    call t14 := Option_unwrap_or(contents#Memory(m)[old_size+12], contents#Memory(m)[old_size+13]);
+    assume is#Integer(t14);
 
-    call tmp := Not(ls[old_size+44]);
-    ls[old_size+45] := tmp;
-
-    tmp := ls[old_size + 45];
-    if (!b#Boolean(tmp)) { goto Label_59; }
+    m := Memory(domain#Memory(m)[old_size+14 := true], contents#Memory(m)[old_size+14 := t14]);
 
     call tmp := LdConst(42);
-    ls[old_size+46] := tmp;
+    m := Memory(domain#Memory(m)[15+old_size := true], contents#Memory(m)[15+old_size := tmp]);
+
+    call tmp := Eq(contents#Memory(m)[old_size+14], contents#Memory(m)[old_size+15]);
+    m := Memory(domain#Memory(m)[16+old_size := true], contents#Memory(m)[16+old_size := tmp]);
+
+    call tmp := Not(contents#Memory(m)[old_size+16]);
+    m := Memory(domain#Memory(m)[17+old_size := true], contents#Memory(m)[17+old_size := tmp]);
+
+    tmp := contents#Memory(m)[old_size + 17];
+if (!b#Boolean(tmp)) { goto Label_23; }
+
+    call tmp := LdConst(10);
+    m := Memory(domain#Memory(m)[18+old_size := true], contents#Memory(m)[18+old_size := tmp]);
 
     assert false;
 
-Label_59:
-    goto Label_74;
+Label_23:
+    return;
 
-Label_60:
-    call tmp := CopyOrMoveValue(ls[old_size+7]);
-    ls[old_size+47] := tmp;
+}
 
-    call tmp := LdConst(20);
-    ls[old_size+48] := tmp;
+procedure Option_test_u64_verify () returns ()
+{
+    call Option_test_u64();
+}
 
-    call tmp := Eq_int(ls[old_size+47], ls[old_size+48]);
-    ls[old_size+49] := tmp;
+procedure {:inline 1} Option_test_append_reverse () returns ()
+{
+    // declare local variables
+    var t0: Value; // Vector_T
+    var t1: Value; // Vector_T
+    var t2: Value; // Vector_T
+    var t3: Value; // Vector_T
+    var t4: Reference; // Vector_T_ref
+    var t5: Value; // Vector_T
+    var t6: Reference; // Vector_T_ref
+    var t7: Value; // bool
+    var t8: Value; // bool
+    var t9: Value; // int
+    var t10: Value; // Vector_T
+    var t11: Reference; // Vector_T_ref
+    var t12: Value; // int
+    var t13: Reference; // Vector_T_ref
+    var t14: Value; // int
+    var t15: Reference; // Vector_T_ref
+    var t16: Reference; // Vector_T_ref
+    var t17: Value; // int
+    var t18: Reference; // Vector_T_ref
+    var t19: Value; // int
+    var t20: Reference; // Vector_T_ref
+    var t21: Value; // Vector_T
+    var t22: Reference; // Vector_T_ref
+    var t23: Value; // bool
+    var t24: Value; // bool
+    var t25: Value; // bool
+    var t26: Value; // int
+    var t27: Reference; // Vector_T_ref
+    var t28: Value; // int
+    var t29: Value; // int
+    var t30: Value; // bool
+    var t31: Value; // bool
+    var t32: Value; // int
+    var t33: Reference; // Vector_T_ref
+    var t34: Value; // int
+    var t35: Reference; // int_ref
+    var t36: Value; // int
+    var t37: Value; // int
+    var t38: Value; // bool
+    var t39: Value; // bool
+    var t40: Value; // int
+    var t41: Reference; // Vector_T_ref
+    var t42: Value; // int
+    var t43: Reference; // int_ref
+    var t44: Value; // int
+    var t45: Value; // int
+    var t46: Value; // bool
+    var t47: Value; // bool
+    var t48: Value; // int
+    var t49: Reference; // Vector_T_ref
+    var t50: Value; // int
+    var t51: Reference; // int_ref
+    var t52: Value; // int
+    var t53: Value; // int
+    var t54: Value; // bool
+    var t55: Value; // bool
+    var t56: Value; // int
+    var t57: Reference; // Vector_T_ref
+    var t58: Value; // int
+    var t59: Reference; // int_ref
+    var t60: Value; // int
+    var t61: Value; // int
+    var t62: Value; // bool
+    var t63: Value; // bool
+    var t64: Value; // int
 
-    call tmp := Not(ls[old_size+49]);
-    ls[old_size+50] := tmp;
+    var tmp: Value;
+    var old_size: int;
+    assume !abort_flag;
 
-    tmp := ls[old_size + 50];
-    if (!b#Boolean(tmp)) { goto Label_67; }
+    // assume arguments are of correct types
 
-    call tmp := LdConst(42);
-    ls[old_size+51] := tmp;
+    old_size := m_size;
+    m_size := m_size + 65;
+
+    // bytecode translation starts here
+    call t2 := Vector_empty();
+    assume is#Vector(t2);
+
+    m := Memory(domain#Memory(m)[old_size+2 := true], contents#Memory(m)[old_size+2 := t2]);
+
+    call tmp := CopyOrMoveValue(contents#Memory(m)[old_size+2]);
+    m := Memory(domain#Memory(m)[0+old_size := true], contents#Memory(m)[0+old_size := tmp]);
+
+    call t3 := Vector_empty();
+    assume is#Vector(t3);
+
+    m := Memory(domain#Memory(m)[old_size+3 := true], contents#Memory(m)[old_size+3 := t3]);
+
+    call tmp := CopyOrMoveValue(contents#Memory(m)[old_size+3]);
+    m := Memory(domain#Memory(m)[1+old_size := true], contents#Memory(m)[1+old_size := tmp]);
+
+    call t4 := BorrowLoc(old_size+0);
+
+    call tmp := CopyOrMoveValue(contents#Memory(m)[old_size+1]);
+    m := Memory(domain#Memory(m)[5+old_size := true], contents#Memory(m)[5+old_size := tmp]);
+
+    call Vector_append(t4, contents#Memory(m)[old_size+5]);
+
+    call t6 := BorrowLoc(old_size+0);
+
+    call t7 := Vector_is_empty(t6);
+    assume is#Boolean(t7);
+
+    m := Memory(domain#Memory(m)[old_size+7 := true], contents#Memory(m)[old_size+7 := t7]);
+
+    call tmp := Not(contents#Memory(m)[old_size+7]);
+    m := Memory(domain#Memory(m)[8+old_size := true], contents#Memory(m)[8+old_size := tmp]);
+
+    tmp := contents#Memory(m)[old_size + 8];
+if (!b#Boolean(tmp)) { goto Label_13; }
+
+    call tmp := LdConst(3);
+    m := Memory(domain#Memory(m)[9+old_size := true], contents#Memory(m)[9+old_size := tmp]);
+
+    assert false;
+
+Label_13:
+    call t10 := Vector_empty();
+    assume is#Vector(t10);
+
+    m := Memory(domain#Memory(m)[old_size+10 := true], contents#Memory(m)[old_size+10 := t10]);
+
+    call tmp := CopyOrMoveValue(contents#Memory(m)[old_size+10]);
+    m := Memory(domain#Memory(m)[1+old_size := true], contents#Memory(m)[1+old_size := tmp]);
+
+    call t11 := BorrowLoc(old_size+1);
+
+    call tmp := LdConst(1);
+    m := Memory(domain#Memory(m)[12+old_size := true], contents#Memory(m)[12+old_size := tmp]);
+
+    call Vector_push_back(t11, contents#Memory(m)[old_size+12]);
+
+    call t13 := BorrowLoc(old_size+1);
+
+    call tmp := LdConst(2);
+    m := Memory(domain#Memory(m)[14+old_size := true], contents#Memory(m)[14+old_size := tmp]);
+
+    call Vector_push_back(t13, contents#Memory(m)[old_size+14]);
+
+    call t15 := BorrowLoc(old_size+1);
+
+    call Vector_reverse(t15);
+
+    call t16 := BorrowLoc(old_size+1);
+
+    call tmp := LdConst(3);
+    m := Memory(domain#Memory(m)[17+old_size := true], contents#Memory(m)[17+old_size := tmp]);
+
+    call Vector_push_back(t16, contents#Memory(m)[old_size+17]);
+
+    call t18 := BorrowLoc(old_size+0);
+
+    call tmp := LdConst(4);
+    m := Memory(domain#Memory(m)[19+old_size := true], contents#Memory(m)[19+old_size := tmp]);
+
+    call Vector_push_back(t18, contents#Memory(m)[old_size+19]);
+
+    call t20 := BorrowLoc(old_size+0);
+
+    call tmp := CopyOrMoveValue(contents#Memory(m)[old_size+1]);
+    m := Memory(domain#Memory(m)[21+old_size := true], contents#Memory(m)[21+old_size := tmp]);
+
+    call Vector_append(t20, contents#Memory(m)[old_size+21]);
+
+    call t22 := BorrowLoc(old_size+0);
+
+    call t23 := Vector_is_empty(t22);
+    assume is#Boolean(t23);
+
+    m := Memory(domain#Memory(m)[old_size+23 := true], contents#Memory(m)[old_size+23 := t23]);
+
+    call tmp := Not(contents#Memory(m)[old_size+23]);
+    m := Memory(domain#Memory(m)[24+old_size := true], contents#Memory(m)[24+old_size := tmp]);
+
+    call tmp := Not(contents#Memory(m)[old_size+24]);
+    m := Memory(domain#Memory(m)[25+old_size := true], contents#Memory(m)[25+old_size := tmp]);
+
+    tmp := contents#Memory(m)[old_size + 25];
+if (!b#Boolean(tmp)) { goto Label_39; }
+
+    call tmp := LdConst(4);
+    m := Memory(domain#Memory(m)[26+old_size := true], contents#Memory(m)[26+old_size := tmp]);
+
+    assert false;
+
+Label_39:
+    call t27 := BorrowLoc(old_size+0);
+
+    call t28 := Vector_length(t27);
+    assume is#Integer(t28);
+
+    m := Memory(domain#Memory(m)[old_size+28 := true], contents#Memory(m)[old_size+28 := t28]);
+
+    call tmp := LdConst(4);
+    m := Memory(domain#Memory(m)[29+old_size := true], contents#Memory(m)[29+old_size := tmp]);
+
+    call tmp := Eq(contents#Memory(m)[old_size+28], contents#Memory(m)[old_size+29]);
+    m := Memory(domain#Memory(m)[30+old_size := true], contents#Memory(m)[30+old_size := tmp]);
+
+    call tmp := Not(contents#Memory(m)[old_size+30]);
+    m := Memory(domain#Memory(m)[31+old_size := true], contents#Memory(m)[31+old_size := tmp]);
+
+    tmp := contents#Memory(m)[old_size + 31];
+if (!b#Boolean(tmp)) { goto Label_47; }
+
+    call tmp := LdConst(5);
+    m := Memory(domain#Memory(m)[32+old_size := true], contents#Memory(m)[32+old_size := tmp]);
+
+    assert false;
+
+Label_47:
+    call t33 := BorrowLoc(old_size+0);
+
+    call tmp := LdConst(0);
+    m := Memory(domain#Memory(m)[34+old_size := true], contents#Memory(m)[34+old_size := tmp]);
+
+    call t35 := Vector_borrow(t33, contents#Memory(m)[old_size+34]);
+
+    call tmp := ReadRef(t35);
+    assume is#Integer(tmp);
+
+    m := Memory(domain#Memory(m)[36+old_size := true], contents#Memory(m)[36+old_size := tmp]);
+
+    call tmp := LdConst(4);
+    m := Memory(domain#Memory(m)[37+old_size := true], contents#Memory(m)[37+old_size := tmp]);
+
+    call tmp := Eq(contents#Memory(m)[old_size+36], contents#Memory(m)[old_size+37]);
+    m := Memory(domain#Memory(m)[38+old_size := true], contents#Memory(m)[38+old_size := tmp]);
+
+    call tmp := Not(contents#Memory(m)[old_size+38]);
+    m := Memory(domain#Memory(m)[39+old_size := true], contents#Memory(m)[39+old_size := tmp]);
+
+    tmp := contents#Memory(m)[old_size + 39];
+if (!b#Boolean(tmp)) { goto Label_57; }
+
+    call tmp := LdConst(7);
+    m := Memory(domain#Memory(m)[40+old_size := true], contents#Memory(m)[40+old_size := tmp]);
+
+    assert false;
+
+Label_57:
+    call t41 := BorrowLoc(old_size+0);
+
+    call tmp := LdConst(1);
+    m := Memory(domain#Memory(m)[42+old_size := true], contents#Memory(m)[42+old_size := tmp]);
+
+    call t43 := Vector_borrow(t41, contents#Memory(m)[old_size+42]);
+
+    call tmp := ReadRef(t43);
+    assume is#Integer(tmp);
+
+    m := Memory(domain#Memory(m)[44+old_size := true], contents#Memory(m)[44+old_size := tmp]);
+
+    call tmp := LdConst(2);
+    m := Memory(domain#Memory(m)[45+old_size := true], contents#Memory(m)[45+old_size := tmp]);
+
+    call tmp := Eq(contents#Memory(m)[old_size+44], contents#Memory(m)[old_size+45]);
+    m := Memory(domain#Memory(m)[46+old_size := true], contents#Memory(m)[46+old_size := tmp]);
+
+    call tmp := Not(contents#Memory(m)[old_size+46]);
+    m := Memory(domain#Memory(m)[47+old_size := true], contents#Memory(m)[47+old_size := tmp]);
+
+    tmp := contents#Memory(m)[old_size + 47];
+if (!b#Boolean(tmp)) { goto Label_67; }
+
+    call tmp := LdConst(7);
+    m := Memory(domain#Memory(m)[48+old_size := true], contents#Memory(m)[48+old_size := tmp]);
 
     assert false;
 
 Label_67:
-    call tmp := CopyOrMoveValue(ls[old_size+8]);
-    ls[old_size+52] := tmp;
+    call t49 := BorrowLoc(old_size+0);
 
-    call tmp := LdConst(10);
-    ls[old_size+53] := tmp;
+    call tmp := LdConst(2);
+    m := Memory(domain#Memory(m)[50+old_size := true], contents#Memory(m)[50+old_size := tmp]);
 
-    call tmp := Eq_int(ls[old_size+52], ls[old_size+53]);
-    ls[old_size+54] := tmp;
+    call t51 := Vector_borrow(t49, contents#Memory(m)[old_size+50]);
 
-    call tmp := Not(ls[old_size+54]);
-    ls[old_size+55] := tmp;
+    call tmp := ReadRef(t51);
+    assume is#Integer(tmp);
 
-    tmp := ls[old_size + 55];
-    if (!b#Boolean(tmp)) { goto Label_74; }
+    m := Memory(domain#Memory(m)[52+old_size := true], contents#Memory(m)[52+old_size := tmp]);
 
-    call tmp := LdConst(42);
-    ls[old_size+56] := tmp;
+    call tmp := LdConst(1);
+    m := Memory(domain#Memory(m)[53+old_size := true], contents#Memory(m)[53+old_size := tmp]);
+
+    call tmp := Eq(contents#Memory(m)[old_size+52], contents#Memory(m)[old_size+53]);
+    m := Memory(domain#Memory(m)[54+old_size := true], contents#Memory(m)[54+old_size := tmp]);
+
+    call tmp := Not(contents#Memory(m)[old_size+54]);
+    m := Memory(domain#Memory(m)[55+old_size := true], contents#Memory(m)[55+old_size := tmp]);
+
+    tmp := contents#Memory(m)[old_size + 55];
+if (!b#Boolean(tmp)) { goto Label_77; }
+
+    call tmp := LdConst(8);
+    m := Memory(domain#Memory(m)[56+old_size := true], contents#Memory(m)[56+old_size := tmp]);
 
     assert false;
 
-Label_74:
+Label_77:
+    call t57 := BorrowLoc(old_size+0);
+
+    call tmp := LdConst(3);
+    m := Memory(domain#Memory(m)[58+old_size := true], contents#Memory(m)[58+old_size := tmp]);
+
+    call t59 := Vector_borrow(t57, contents#Memory(m)[old_size+58]);
+
+    call tmp := ReadRef(t59);
+    assume is#Integer(tmp);
+
+    m := Memory(domain#Memory(m)[60+old_size := true], contents#Memory(m)[60+old_size := tmp]);
+
+    call tmp := LdConst(3);
+    m := Memory(domain#Memory(m)[61+old_size := true], contents#Memory(m)[61+old_size := tmp]);
+
+    call tmp := Eq(contents#Memory(m)[old_size+60], contents#Memory(m)[old_size+61]);
+    m := Memory(domain#Memory(m)[62+old_size := true], contents#Memory(m)[62+old_size := tmp]);
+
+    call tmp := Not(contents#Memory(m)[old_size+62]);
+    m := Memory(domain#Memory(m)[63+old_size := true], contents#Memory(m)[63+old_size := tmp]);
+
+    tmp := contents#Memory(m)[old_size + 63];
+if (!b#Boolean(tmp)) { goto Label_87; }
+
+    call tmp := LdConst(9);
+    m := Memory(domain#Memory(m)[64+old_size := true], contents#Memory(m)[64+old_size := tmp]);
+
+    assert false;
+
+Label_87:
     return;
 
+}
+
+procedure Option_test_append_reverse_verify () returns ()
+{
+    call Option_test_append_reverse();
+}
+
+procedure {:inline 1} Option_test_get_set_swap () returns ()
+{
+    // declare local variables
+    var t0: Value; // Vector_T
+    var t1: Value; // Vector_T
+    var t2: Value; // Vector_T
+    var t3: Value; // Vector_T
+    var t4: Value; // Vector_T
+    var t5: Reference; // Vector_T_ref
+    var t6: Value; // int
+    var t7: Reference; // Vector_T_ref
+    var t8: Value; // int
+    var t9: Reference; // Vector_T_ref
+    var t10: Value; // int
+    var t11: Value; // int
+    var t12: Reference; // Vector_T_ref
+    var t13: Value; // int
+    var t14: Value; // int
+    var t15: Value; // int
+    var t16: Value; // bool
+    var t17: Value; // bool
+    var t18: Value; // int
+    var t19: Reference; // Vector_T_ref
+    var t20: Value; // int
+    var t21: Reference; // Vector_T_ref
+    var t22: Value; // int
+    var t23: Value; // int
+    var t24: Reference; // Vector_T_ref
+    var t25: Value; // int
+    var t26: Value; // int
+    var t27: Value; // int
+    var t28: Value; // bool
+    var t29: Value; // bool
+    var t30: Value; // int
+    var t31: Reference; // Vector_T_ref
+    var t32: Value; // int
+    var t33: Value; // int
+    var t34: Value; // int
+    var t35: Value; // bool
+    var t36: Value; // bool
+    var t37: Value; // int
+    var t38: Reference; // Vector_T_ref
+    var t39: Value; // int
+    var t40: Value; // int
+    var t41: Reference; // Vector_T_ref
+    var t42: Value; // int
+    var t43: Value; // int
+    var t44: Value; // int
+    var t45: Value; // bool
+    var t46: Value; // bool
+    var t47: Value; // int
+    var t48: Reference; // Vector_T_ref
+    var t49: Value; // int
+    var t50: Value; // int
+    var t51: Value; // int
+    var t52: Value; // bool
+    var t53: Value; // bool
+    var t54: Value; // int
+    var t55: Reference; // Vector_T_ref
+    var t56: Value; // int
+    var t57: Value; // int
+    var t58: Value; // bool
+    var t59: Value; // bool
+    var t60: Value; // int
+    var t61: Reference; // Vector_T_ref
+    var t62: Value; // int
+    var t63: Value; // int
+    var t64: Value; // bool
+    var t65: Value; // bool
+    var t66: Value; // int
+    var t67: Reference; // Vector_T_ref
+    var t68: Value; // int
+    var t69: Value; // int
+    var t70: Value; // bool
+    var t71: Value; // bool
+    var t72: Value; // int
+    var t73: Reference; // Vector_T_ref
+    var t74: Value; // bool
+    var t75: Value; // bool
+    var t76: Value; // int
+    var t77: Value; // Vector_T
+
+    var tmp: Value;
+    var old_size: int;
+    assume !abort_flag;
+
+    // assume arguments are of correct types
+
+    old_size := m_size;
+    m_size := m_size + 78;
+
+    // bytecode translation starts here
+    call t2 := Vector_empty();
+    assume is#Vector(t2);
+
+    m := Memory(domain#Memory(m)[old_size+2 := true], contents#Memory(m)[old_size+2 := t2]);
+
+    call tmp := CopyOrMoveValue(contents#Memory(m)[old_size+2]);
+    m := Memory(domain#Memory(m)[0+old_size := true], contents#Memory(m)[0+old_size := tmp]);
+
+    call tmp := CopyOrMoveValue(contents#Memory(m)[old_size+0]);
+    m := Memory(domain#Memory(m)[3+old_size := true], contents#Memory(m)[3+old_size := tmp]);
+
+    call Vector_destroy_empty(contents#Memory(m)[old_size+3]);
+
+    call t4 := Vector_empty();
+    assume is#Vector(t4);
+
+    m := Memory(domain#Memory(m)[old_size+4 := true], contents#Memory(m)[old_size+4 := t4]);
+
+    call tmp := CopyOrMoveValue(contents#Memory(m)[old_size+4]);
+    m := Memory(domain#Memory(m)[1+old_size := true], contents#Memory(m)[1+old_size := tmp]);
+
+    call t5 := BorrowLoc(old_size+1);
+
+    call tmp := LdConst(1);
+    m := Memory(domain#Memory(m)[6+old_size := true], contents#Memory(m)[6+old_size := tmp]);
+
+    call Vector_push_back(t5, contents#Memory(m)[old_size+6]);
+
+    call t7 := BorrowLoc(old_size+1);
+
+    call tmp := LdConst(2);
+    m := Memory(domain#Memory(m)[8+old_size := true], contents#Memory(m)[8+old_size := tmp]);
+
+    call Vector_push_back(t7, contents#Memory(m)[old_size+8]);
+
+    call t9 := BorrowLoc(old_size+1);
+
+    call tmp := LdConst(1);
+    m := Memory(domain#Memory(m)[10+old_size := true], contents#Memory(m)[10+old_size := tmp]);
+
+    call tmp := LdConst(22);
+    m := Memory(domain#Memory(m)[11+old_size := true], contents#Memory(m)[11+old_size := tmp]);
+
+    call Vector_set(t9, contents#Memory(m)[old_size+10], contents#Memory(m)[old_size+11]);
+
+    call t12 := BorrowLoc(old_size+1);
+
+    call tmp := LdConst(1);
+    m := Memory(domain#Memory(m)[13+old_size := true], contents#Memory(m)[13+old_size := tmp]);
+
+    call t14 := Vector_get(t12, contents#Memory(m)[old_size+13]);
+    assume is#Integer(t14);
+
+    m := Memory(domain#Memory(m)[old_size+14 := true], contents#Memory(m)[old_size+14 := t14]);
+
+    call tmp := LdConst(22);
+    m := Memory(domain#Memory(m)[15+old_size := true], contents#Memory(m)[15+old_size := tmp]);
+
+    call tmp := Eq(contents#Memory(m)[old_size+14], contents#Memory(m)[old_size+15]);
+    m := Memory(domain#Memory(m)[16+old_size := true], contents#Memory(m)[16+old_size := tmp]);
+
+    call tmp := Not(contents#Memory(m)[old_size+16]);
+    m := Memory(domain#Memory(m)[17+old_size := true], contents#Memory(m)[17+old_size := tmp]);
+
+    tmp := contents#Memory(m)[old_size + 17];
+if (!b#Boolean(tmp)) { goto Label_25; }
+
+    call tmp := LdConst(42);
+    m := Memory(domain#Memory(m)[18+old_size := true], contents#Memory(m)[18+old_size := tmp]);
+
+    assert false;
+
+Label_25:
+    call t19 := BorrowLoc(old_size+1);
+
+    call tmp := LdConst(3);
+    m := Memory(domain#Memory(m)[20+old_size := true], contents#Memory(m)[20+old_size := tmp]);
+
+    call Vector_push_back(t19, contents#Memory(m)[old_size+20]);
+
+    call t21 := BorrowLoc(old_size+1);
+
+    call tmp := LdConst(1);
+    m := Memory(domain#Memory(m)[22+old_size := true], contents#Memory(m)[22+old_size := tmp]);
+
+    call tmp := LdConst(2);
+    m := Memory(domain#Memory(m)[23+old_size := true], contents#Memory(m)[23+old_size := tmp]);
+
+    call Vector_swap(t21, contents#Memory(m)[old_size+22], contents#Memory(m)[old_size+23]);
+
+    call t24 := BorrowLoc(old_size+1);
+
+    call tmp := LdConst(1);
+    m := Memory(domain#Memory(m)[25+old_size := true], contents#Memory(m)[25+old_size := tmp]);
+
+    call t26 := Vector_get(t24, contents#Memory(m)[old_size+25]);
+    assume is#Integer(t26);
+
+    m := Memory(domain#Memory(m)[old_size+26 := true], contents#Memory(m)[old_size+26 := t26]);
+
+    call tmp := LdConst(3);
+    m := Memory(domain#Memory(m)[27+old_size := true], contents#Memory(m)[27+old_size := tmp]);
+
+    call tmp := Eq(contents#Memory(m)[old_size+26], contents#Memory(m)[old_size+27]);
+    m := Memory(domain#Memory(m)[28+old_size := true], contents#Memory(m)[28+old_size := tmp]);
+
+    call tmp := Not(contents#Memory(m)[old_size+28]);
+    m := Memory(domain#Memory(m)[29+old_size := true], contents#Memory(m)[29+old_size := tmp]);
+
+    tmp := contents#Memory(m)[old_size + 29];
+if (!b#Boolean(tmp)) { goto Label_41; }
+
+    call tmp := LdConst(43);
+    m := Memory(domain#Memory(m)[30+old_size := true], contents#Memory(m)[30+old_size := tmp]);
+
+    assert false;
+
+Label_41:
+    call t31 := BorrowLoc(old_size+1);
+
+    call tmp := LdConst(2);
+    m := Memory(domain#Memory(m)[32+old_size := true], contents#Memory(m)[32+old_size := tmp]);
+
+    call t33 := Vector_get(t31, contents#Memory(m)[old_size+32]);
+    assume is#Integer(t33);
+
+    m := Memory(domain#Memory(m)[old_size+33 := true], contents#Memory(m)[old_size+33 := t33]);
+
+    call tmp := LdConst(22);
+    m := Memory(domain#Memory(m)[34+old_size := true], contents#Memory(m)[34+old_size := tmp]);
+
+    call tmp := Eq(contents#Memory(m)[old_size+33], contents#Memory(m)[old_size+34]);
+    m := Memory(domain#Memory(m)[35+old_size := true], contents#Memory(m)[35+old_size := tmp]);
+
+    call tmp := Not(contents#Memory(m)[old_size+35]);
+    m := Memory(domain#Memory(m)[36+old_size := true], contents#Memory(m)[36+old_size := tmp]);
+
+    tmp := contents#Memory(m)[old_size + 36];
+if (!b#Boolean(tmp)) { goto Label_50; }
+
+    call tmp := LdConst(44);
+    m := Memory(domain#Memory(m)[37+old_size := true], contents#Memory(m)[37+old_size := tmp]);
+
+    assert false;
+
+Label_50:
+    call t38 := BorrowLoc(old_size+1);
+
+    call tmp := LdConst(2);
+    m := Memory(domain#Memory(m)[39+old_size := true], contents#Memory(m)[39+old_size := tmp]);
+
+    call tmp := LdConst(1);
+    m := Memory(domain#Memory(m)[40+old_size := true], contents#Memory(m)[40+old_size := tmp]);
+
+    call Vector_swap(t38, contents#Memory(m)[old_size+39], contents#Memory(m)[old_size+40]);
+
+    call t41 := BorrowLoc(old_size+1);
+
+    call tmp := LdConst(1);
+    m := Memory(domain#Memory(m)[42+old_size := true], contents#Memory(m)[42+old_size := tmp]);
+
+    call t43 := Vector_get(t41, contents#Memory(m)[old_size+42]);
+    assume is#Integer(t43);
+
+    m := Memory(domain#Memory(m)[old_size+43 := true], contents#Memory(m)[old_size+43 := t43]);
+
+    call tmp := LdConst(22);
+    m := Memory(domain#Memory(m)[44+old_size := true], contents#Memory(m)[44+old_size := tmp]);
+
+    call tmp := Eq(contents#Memory(m)[old_size+43], contents#Memory(m)[old_size+44]);
+    m := Memory(domain#Memory(m)[45+old_size := true], contents#Memory(m)[45+old_size := tmp]);
+
+    call tmp := Not(contents#Memory(m)[old_size+45]);
+    m := Memory(domain#Memory(m)[46+old_size := true], contents#Memory(m)[46+old_size := tmp]);
+
+    tmp := contents#Memory(m)[old_size + 46];
+if (!b#Boolean(tmp)) { goto Label_63; }
+
+    call tmp := LdConst(45);
+    m := Memory(domain#Memory(m)[47+old_size := true], contents#Memory(m)[47+old_size := tmp]);
+
+    assert false;
+
+Label_63:
+    call t48 := BorrowLoc(old_size+1);
+
+    call tmp := LdConst(2);
+    m := Memory(domain#Memory(m)[49+old_size := true], contents#Memory(m)[49+old_size := tmp]);
+
+    call t50 := Vector_get(t48, contents#Memory(m)[old_size+49]);
+    assume is#Integer(t50);
+
+    m := Memory(domain#Memory(m)[old_size+50 := true], contents#Memory(m)[old_size+50 := t50]);
+
+    call tmp := LdConst(3);
+    m := Memory(domain#Memory(m)[51+old_size := true], contents#Memory(m)[51+old_size := tmp]);
+
+    call tmp := Eq(contents#Memory(m)[old_size+50], contents#Memory(m)[old_size+51]);
+    m := Memory(domain#Memory(m)[52+old_size := true], contents#Memory(m)[52+old_size := tmp]);
+
+    call tmp := Not(contents#Memory(m)[old_size+52]);
+    m := Memory(domain#Memory(m)[53+old_size := true], contents#Memory(m)[53+old_size := tmp]);
+
+    tmp := contents#Memory(m)[old_size + 53];
+if (!b#Boolean(tmp)) { goto Label_72; }
+
+    call tmp := LdConst(46);
+    m := Memory(domain#Memory(m)[54+old_size := true], contents#Memory(m)[54+old_size := tmp]);
+
+    assert false;
+
+Label_72:
+    call t55 := BorrowLoc(old_size+1);
+
+    call t56 := Vector_pop_back(t55);
+    assume is#Integer(t56);
+
+    m := Memory(domain#Memory(m)[old_size+56 := true], contents#Memory(m)[old_size+56 := t56]);
+
+    call tmp := LdConst(3);
+    m := Memory(domain#Memory(m)[57+old_size := true], contents#Memory(m)[57+old_size := tmp]);
+
+    call tmp := Eq(contents#Memory(m)[old_size+56], contents#Memory(m)[old_size+57]);
+    m := Memory(domain#Memory(m)[58+old_size := true], contents#Memory(m)[58+old_size := tmp]);
+
+    call tmp := Not(contents#Memory(m)[old_size+58]);
+    m := Memory(domain#Memory(m)[59+old_size := true], contents#Memory(m)[59+old_size := tmp]);
+
+    tmp := contents#Memory(m)[old_size + 59];
+if (!b#Boolean(tmp)) { goto Label_80; }
+
+    call tmp := LdConst(47);
+    m := Memory(domain#Memory(m)[60+old_size := true], contents#Memory(m)[60+old_size := tmp]);
+
+    assert false;
+
+Label_80:
+    call t61 := BorrowLoc(old_size+1);
+
+    call t62 := Vector_pop_back(t61);
+    assume is#Integer(t62);
+
+    m := Memory(domain#Memory(m)[old_size+62 := true], contents#Memory(m)[old_size+62 := t62]);
+
+    call tmp := LdConst(22);
+    m := Memory(domain#Memory(m)[63+old_size := true], contents#Memory(m)[63+old_size := tmp]);
+
+    call tmp := Eq(contents#Memory(m)[old_size+62], contents#Memory(m)[old_size+63]);
+    m := Memory(domain#Memory(m)[64+old_size := true], contents#Memory(m)[64+old_size := tmp]);
+
+    call tmp := Not(contents#Memory(m)[old_size+64]);
+    m := Memory(domain#Memory(m)[65+old_size := true], contents#Memory(m)[65+old_size := tmp]);
+
+    tmp := contents#Memory(m)[old_size + 65];
+if (!b#Boolean(tmp)) { goto Label_88; }
+
+    call tmp := LdConst(48);
+    m := Memory(domain#Memory(m)[66+old_size := true], contents#Memory(m)[66+old_size := tmp]);
+
+    assert false;
+
+Label_88:
+    call t67 := BorrowLoc(old_size+1);
+
+    call t68 := Vector_pop_back(t67);
+    assume is#Integer(t68);
+
+    m := Memory(domain#Memory(m)[old_size+68 := true], contents#Memory(m)[old_size+68 := t68]);
+
+    call tmp := LdConst(1);
+    m := Memory(domain#Memory(m)[69+old_size := true], contents#Memory(m)[69+old_size := tmp]);
+
+    call tmp := Eq(contents#Memory(m)[old_size+68], contents#Memory(m)[old_size+69]);
+    m := Memory(domain#Memory(m)[70+old_size := true], contents#Memory(m)[70+old_size := tmp]);
+
+    call tmp := Not(contents#Memory(m)[old_size+70]);
+    m := Memory(domain#Memory(m)[71+old_size := true], contents#Memory(m)[71+old_size := tmp]);
+
+    tmp := contents#Memory(m)[old_size + 71];
+if (!b#Boolean(tmp)) { goto Label_96; }
+
+    call tmp := LdConst(49);
+    m := Memory(domain#Memory(m)[72+old_size := true], contents#Memory(m)[72+old_size := tmp]);
+
+    assert false;
+
+Label_96:
+    call t73 := BorrowLoc(old_size+1);
+
+    call t74 := Vector_is_empty(t73);
+    assume is#Boolean(t74);
+
+    m := Memory(domain#Memory(m)[old_size+74 := true], contents#Memory(m)[old_size+74 := t74]);
+
+    call tmp := Not(contents#Memory(m)[old_size+74]);
+    m := Memory(domain#Memory(m)[75+old_size := true], contents#Memory(m)[75+old_size := tmp]);
+
+    tmp := contents#Memory(m)[old_size + 75];
+if (!b#Boolean(tmp)) { goto Label_102; }
+
+    call tmp := LdConst(50);
+    m := Memory(domain#Memory(m)[76+old_size := true], contents#Memory(m)[76+old_size := tmp]);
+
+    assert false;
+
+Label_102:
+    call tmp := CopyOrMoveValue(contents#Memory(m)[old_size+1]);
+    m := Memory(domain#Memory(m)[77+old_size := true], contents#Memory(m)[77+old_size := tmp]);
+
+    call Vector_destroy_empty(contents#Memory(m)[old_size+77]);
+
+    return;
+
+}
+
+procedure Option_test_get_set_swap_verify () returns ()
+{
+    call Option_test_get_set_swap();
 }
